LeanDag.lean
@@ -75,6 +75,7 @@ import LeanDag.Integration.Hydrozoan.ChopDecided
 import LeanDag.Integration.Hydrozoan.FillDecided
 import LeanDag.Integration.Hydrozoan.Stack
 import LeanDag.Integration.Hydrozoan.Liveness
+import LeanDag.Integration.Hydrozoan.Deployment
 import LeanDag.SafeSkip.Basic
 import LeanDag.SafeSkip.Invariance
 import LeanDag.SafeSkip.Jump
